src/FcEtt/fc_consist.v
@@ -18,14 +18,13 @@ Require Import FcEtt.fc_head_reduction.
 (* Needed for annotation lemma at end. *)
 Require Import FcEtt.fc_preservation.
 Require Import FcEtt.ext_subst.
-Require Import FcEtt.ext_invert.
 
 Set Implicit Arguments.
 Set Bullet Behavior "Strict Subproofs".
 
 
 Module fc_consist (wf : fc_wf_sig) (weak : fc_weak_sig) (subst : fc_subst_sig)
-                  (e_subst : ext_subst_sig).
+                  (e_invert : ext_invert_sig)(e_subst : ext_subst_sig).
 
 Import wf weak.
 
@@ -35,20 +34,21 @@ Export subst.
 Module invert := fc_invert wf weak subst.
 Export invert.
 
-Module e_invert := ext_invert e_subst.
-Import e_invert.
 
 Module consist := ext_consist e_invert wf.
 Export consist.
 
+
 Module erase' := erase wf weak subst e_invert.
 Export erase'.
+
 
 Module head := fc_head_reduction  e_invert weak wf subst.
 Export head.
 
 Module pres := fc_preservation wf weak subst e_subst.
 Import pres.
+(* Why does this cause so many messages? *)
 
 Definition AnnGood G D := Good (erase_context G) D.
 
@@ -79,27 +79,76 @@ Proof.
 Qed.
 
 
+Lemma Paths_are_DataTy : forall T a,
+    Path T a -> Value a -> forall G A, AnnTyping G a A -> DataTy A a_Star.
+Proof.
+  induction 1; intros.
+  - inversion H0. subst.
+    eapply (binds_to_type _ _ AnnSig_an_toplevel); eauto.
+  - inversion H1. inversion H2. subst.
+    move: (IHPath H8 _ _ H14) => h0.
+    inversion h0. subst.
+    pick fresh x.
+    rewrite (tm_subst_tm_tm_intro x); eauto with lngen.
+  - inversion H1. inversion H2. subst.
+    move: (IHPath H7 _ _ H11) => h0.
+    inversion h0. subst.
+    pick fresh x.
+    rewrite (co_subst_co_tm_intro x); eauto with lngen.
+  - inversion H1.
+Qed.
+
+
+
+Lemma Paths_have_value_types : forall T a,
+    Path T a -> Value a -> forall G A, AnnTyping G a A -> value_type A.
+Proof. intros.
+       eapply DataTy_value_type; eauto.
+       eapply Paths_are_DataTy; eauto.
+Qed.
+
+Lemma values_have_value_types :
+  forall G D a A, AnnGood G D ->  AnnTyping G a A -> Value a -> value_type A.
+Proof.
+  intros G D a A AN H V.
+  move: (AnnTyping_regularity H) => h0.
+  inversion H; subst; auto.
+  all: try solve [inversion V; inversion H2].
+  all: match goal with
+  | [H : AnnTyping ?G ?b ?A |- value_type ?b] =>
+    apply AnnTyping_lc in H; split_hyp; lc_inversion c;  eauto
+       end.
+  + inversion V.
+    eapply (@Paths_have_value_types T (a_App b rho a0)); eauto.
+  + inversion V.
+    eapply (@Paths_have_value_types T (a_CApp a1 g)); eauto.
+  + eapply DataTy_value_type.
+    eapply (binds_to_type _ _ AnnSig_an_toplevel); eauto.
+Qed.
+
 
 (* --------- Paths infect the cannonical forms lemmas for functions --------- *)
 
 Lemma canonical_forms_a_Pi :
   forall G D a rho A B, AnnGood G D ->
                    AnnTyping G a (a_Pi rho A B) -> Value a ->
-                   (exists a', a = a_Abs rho A a').
+                   (exists a', a = a_Abs rho A a') \/ (exists T, Path T a).
 Proof.
   intros G D a rho A B AN H V.
   inversion V; subst; inversion H; subst; try solve [inversion H0].
-  all: try solve [exists a0; eauto].
+  all: try solve [left; exists a0; auto].
+  all: try solve [right; exists T; auto].
 Qed.
 
 Lemma canonical_forms_a_CPi :
   forall G D a phi B, AnnGood G D ->
                  AnnTyping G a (a_CPi phi B) -> Value a ->
-                 (exists a', a = a_CAbs phi a').
+                 (exists a', a = a_CAbs phi a') \/ (exists T, Path T a).
 Proof.
   intros G D a phi B AN H V.
   inversion V; subst; inversion H; subst; try solve [inversion H0].
-  all: try solve [exists a0; auto].
+  all: try solve [left; exists a0; auto].
+  all: try solve [right; exists T; auto].
 Qed.
 
 Lemma consistent_a_Pi :
@@ -115,6 +164,7 @@ Proof.
   - subst. exists C1. exists C2. auto.
   - inversion VT.
   - inversion VT.
+  - inversion H0.
   - assert False.
     apply AnnDefEq_lc in DE. split_hyp.
     match goal with
@@ -139,6 +189,7 @@ Proof.
   destruct C; try destruct rho; simpl in H; inversion H;
   try solve [inversion VT; inversion H1].
   - subst. exists phi0. exists C.  auto.
+  - inversion H0.
   - assert False.
     apply AnnDefEq_lc in DE. split_hyp.
     apply H0. econstructor.
@@ -150,23 +201,14 @@ Proof.
     apply value_type_erase in VT. done.
 Qed.
 
-Lemma values_have_value_types :
-  forall G D a A, AnnGood G D ->  AnnTyping G a A -> Value a -> value_type A.
-Proof.
-  intros G D a A AN H V.
-  move: (AnnTyping_regularity H) => h0.
-  inversion H; subst; auto.
-  all: try solve [inversion V; inversion H2].
-  all: match goal with
-  | [H : AnnTyping ?G ?b ?A |- value_type ?b] =>
-    apply AnnTyping_lc in H; split_hyp; lc_inversion c;  eauto
-       end.
-Qed.
-
 
 Definition irrelevant G D (a : tm) :=
   (forall x A, binds x (Tm A) G -> x `notin` fv_tm (erase a)) /\ AnnGood G D.
 
+
+(* Other statement?
+Lemma progress : forall a A G D, AnnGood G D -> AnnTyping G a A -> CoercedValue a \/ exists a', head_reduction G a a'.
+*)
 Lemma progress : forall G a A, irrelevant G (dom G) a -> AnnTyping G a A -> CoercedValue a \/ exists a', head_reduction G a a'.
 Proof.
   intros G a A AN H.
@@ -218,7 +260,7 @@ Proof.
         H: CoercedValue b |- _ => inversion H
       end.
       -- (* application of a value *)
-        edestruct canonical_forms_a_Pi as [ a1 EQ] ; eauto; subst.
+        edestruct canonical_forms_a_Pi as [[ a1 EQ] | [T P]] ; eauto; subst.
         (* path case solved automatically *)
         ++ right. (* a lambda, do a beta reduction *)
            exists (open_tm_wrt_tm a1 a). eapply An_AppAbs; eauto.
@@ -228,7 +270,7 @@ Proof.
          subst.
          have VT: value_type A1. eapply values_have_value_types; eauto.
          edestruct consistent_a_Pi as (A' & B' & EQ); eauto. subst.
-         edestruct canonical_forms_a_Pi as [ a0' EQ]; eauto; subst.
+         edestruct canonical_forms_a_Pi as [[ a0' EQ] | [T P]]; eauto; subst.
     + subst.
       match goal with H : exists a' : tm, head_reduction G b a' |- _ => destruct H end.
       right. eexists. eapply An_AppLeft; eauto.
@@ -247,17 +289,25 @@ Proof.
       match goal with
         H : CoercedValue ?a1 |- _ => inversion H
       end.
-      -- edestruct canonical_forms_a_CPi as [a2 EQ]; eauto; subst.
+      -- edestruct canonical_forms_a_CPi as [[a2 EQ]|[T p]]; eauto; subst.
          right. exists (open_tm_wrt_co a2 g). eapply An_CAppCAbs; eauto.
          destruct (AnnTyping_lc H) as [h0 h1]. inversion h0; auto.
       -- subst.  inversion H. subst.
          have VT: value_type A. eapply values_have_value_types; eauto.
         edestruct consistent_a_CPi as (A' & a2 & EQ); eauto. subst.
-        edestruct canonical_forms_a_CPi as [a0' EQ]; eauto; subst.
+        edestruct canonical_forms_a_CPi as [[a0' EQ]|[T p]]; eauto; subst.
     + destruct H5. right. eexists. eapply An_CAppLeft. eauto. eauto.
+  - left. eauto.
   - right. exists a. eauto.
 Qed.
 
+
+(* ------------------------------------- *)
+
+(* This is proved in the preservation file.
+Lemma reduction_erasure : forall G a a',
+    head_reduction G a a' ->
+    reduction_in_one (erase a) (erase a') \/ erase a = erase a'. *)
 
 
 (* ------------------------------------- *)
@@ -447,6 +497,48 @@ Proof.
   + destruct rho; simpl in V; inversion V; subst;
     move: (IHAnnTyping1 GG (erase b) eq_refl ltac:(auto)) => [av [MS [CV EE]]];
     inversion CV; subst.
+    ++ exists (a_App av Rel a).
+       repeat split. eapply multi_An_AppLeft; eauto_lc.
+       repeat econstructor; eauto_lc.
+       eapply Path_to_Path; eauto_lc.
+       simpl. autorewcs. congruence.
+    ++ move: (multi_preservation MS H) => TC. inversion TC.
+       move: (values_have_value_types GG H9 H3) => VT.
+       move: (consistent_a_Pi GG VT H11) => [A' [B' EQ]]. subst.
+       pose VV := H3. clearbody VV.
+       eapply An_Push with (b:=a) in H3; try eapply H11; try reflexivity.
+       eexists.
+       split. eapply multi_trans.
+       eapply multi_An_AppLeft; eauto_lc.
+       eapply multi_step; eauto_lc.
+       eapply multi_refl; eauto_lc.
+       repeat econstructor; eauto_lc.
+       split.
+       eapply CC; econstructor; eauto_lc.
+       econstructor; eauto_lc.
+       eapply Path_to_Path; eauto_lc.
+       simpl in EE. simpl. congruence.
+    ++ exists (a_App av Irrel a).
+       repeat split. eapply multi_An_AppLeft; eauto_lc.
+       repeat econstructor; eauto_lc.
+       eapply Path_to_Path; eauto_lc.
+       simpl. autorewcs. congruence.
+    ++ move: (multi_preservation MS H) => TC. inversion TC.
+       move: (values_have_value_types GG H9 H3) => VT.
+       move: (consistent_a_Pi GG VT H11) => [A' [B' EQ]]. subst.
+       pose VV := H3. clearbody VV.
+       eapply An_Push with (b:=a) in H3; try eapply H11; try reflexivity.
+       eexists.
+       split. eapply multi_trans.
+       eapply multi_An_AppLeft; eauto_lc.
+       eapply multi_step; eauto_lc.
+       eapply multi_refl; eauto_lc.
+       repeat econstructor; eauto_lc.
+       split.
+       eapply CC; econstructor; eauto_lc.
+       econstructor; eauto_lc.
+       eapply Path_to_Path; eauto_lc.
+       simpl in EE. simpl. congruence.
 
   + move: (IHAnnTyping1 GG _ eq_refl V) => [av [MS [CV EE]]].
     inversion CV.
@@ -478,6 +570,32 @@ Proof.
     repeat split; try eapply multi_refl; eauto using Value_lc;
       simpl; auto.
     econstructor; eauto using AnnTyping_lc1, AnnPropWff_lc.
+  + (* CApp case (for paths) *)
+    simpl in V; inversion V; subst;
+    move: (IHAnnTyping GG (erase a1) eq_refl ltac:(auto)) => [av [MS [CV EE]]];
+    inversion CV; subst.
+    ++ exists (a_CApp av g).
+       repeat split.
+       eapply multi_An_CAppLeft; eauto_lc.
+       repeat econstructor; eauto_lc.
+       eapply Path_to_Path; eauto_lc.
+       simpl. autorewcs. congruence.
+    ++ move: (multi_preservation MS H) => TC. inversion TC.
+       move: (values_have_value_types GG H9 H3) => VT.
+       move: (consistent_a_CPi GG VT H11) => [A' [B' EQ]]. subst.
+       pose VV := H3. clearbody VV.
+       eapply An_CPush with (g:=g0) in H3; try eapply H11; try reflexivity.
+       eexists.
+       split.
+       eapply multi_trans.
+       eapply multi_An_CAppLeft; eauto_lc.
+       eapply multi_step; eauto_lc.
+       eapply multi_refl; eauto_lc.
+       repeat econstructor; eauto_lc.
+       split.
+       eapply CC; econstructor; eauto_lc.
+       eapply Path_to_Path; eauto_lc.
+       simpl in EE. simpl. congruence.
 Qed.
 
 
@@ -492,6 +610,22 @@ Ltac solve_irrelevant y AA b0 h0 :=
     try (intros y AA b0; move: (H4 y AA b0) => h0; fsetdec) end.
 
 
+(* paths are not (erased) abstractions. *)
+Lemma paths_arent_abs :
+  forall a T, Path T a -> forall rho b, a = a_UAbs rho b -> False.
+Proof.
+  intros a T P.
+  induction P; intros r b0 EQ;
+    try  destruct rho; simpl in *; inversion EQ.
+Qed.
+
+Ltac no_paths:=
+  match goal with
+    [ EE : erase (a_App ?b0 ?rho ?a) = a_UAbs _ ?b, H : Path ?T ?b0 |- _ ] =>
+    destruct rho; simpl in EE;
+    match goal with
+      [ FF : ?a = a_UAbs _ ?b |- _ ] =>
+      have P: (Path T a); by eauto using lc_tm_erase end end.
 
 (* Each of the subcases are by induction on a0 to account for top-level coercions on the term.
    This tactic handles all of the inductive cases. *)
@@ -630,6 +764,8 @@ Proof.
            rewrite (tm_subst_tm_tm_intro y); auto.
            eapply tm_subst_tm_tm_lc_tm; eauto using AnnTyping_lc1. }
          rewrite open_tm_erase_tm. auto.
+         (* prove that paths don't erase to abstractions. *)
+         no_paths.
       ++ (* av = (a |> g) *)
          have LC: lc_tm a0_1 by eauto using AnnTyping_lc1.
          (* Push rule *)
@@ -676,6 +812,11 @@ Proof.
          (* erasure property *)
          simpl_erase. auto.
 
+         destruct rho.
+         +++ have P: Path T (a_App (erase v) Rel (erase a0)); by eauto
+                                                                    using lc_tm_erase.
+         +++ have P: Path T (a_App (erase v) Irrel a_Bullet); by eauto using lc_tm_erase.
+
     + (* No coercions. a0 is a direct (Irrel) application of
         a0_1, which erases to an abstraction. *)
       destruct rho0; simpl in H3; inversion H3.
@@ -721,6 +862,7 @@ Proof.
            apply fv_tm_erase_tm; auto.
          }
 
+         no_paths.
       ++ (* av = (a |> g) *)
          have LC: lc_tm a0_1 by eauto using AnnTyping_lc1.
          (* Push rule *)
@@ -788,6 +930,10 @@ Proof.
            apply fv_tm_erase_tm; auto.
          }
 
+         destruct rho.
+         +++ have P: Path T (a_App (erase v) Rel (erase a0)); by eauto
+                                                                    using lc_tm_erase.
+         +++ have P: Path T (a_App (erase v) Irrel a_Bullet); by eauto using lc_tm_erase.
 
     + (* induction step for top-level coercions (Rel) *)
       induction_a0.
